src/smtencoding/FStar.SMTEncoding.Env.fst
@@ -206,6 +206,9 @@ let fresh_fvar mname x s = let xsym = varops.fresh mname x in xsym, mkFreeV <| m
 let gen_term_var (env:env_t) (x:bv) =
     let ysym = "@x"^(string_of_int env.depth) in
     let y = mkFreeV <| mk_fv (ysym, Term_sort) in
+    (* Note: the encoding of impure function arrows (among other places
+    probably) relies on the fact that this is exactly a FreeV. See getfreeV in
+    FStar.SMTEncoding.EncodeTerm.fst *)
     ysym, y, {env with bvar_bindings=add_bvar_binding (x, y) env.bvar_bindings
                      ; tcenv = Env.push_bv env.tcenv x
                      ; depth = env.depth + 1 }
